verify.dfy
@@ -8,11 +8,11 @@ module verify {
   import opened tls_wrapper
 
   method main() {
-    var sock := new Socket;
     var privateKey := "privateKey";
     var hostname := "hostname";
-
-    sock.Init(256, privateKey, hostname);
+    var sock := new Socket.Init(256, privateKey, hostname);
+  
+    // sock.Init(256, privateKey, hostname);
     // assert all properties
     assert sock.privateKey == "privateKey";
     assert sock.remHostname == hostname;
@@ -20,19 +20,18 @@ module verify {
     assert fresh(sock.cipherSuites);
 
     //call set_cert_chain
-    var conn_ctx := new tls_conn_ctx;
-    conn_ctx.Init();
-    var tls_seq := new tls_opts_seq;
-    tls_seq.Init();
+    var conn_ctx := new tls_conn_ctx.Init();
+    var tls_seq := new tls_opts_seq.Init();
     // add tls_opts_client_setup - in connect cb
     // connect_cb()
     var y := set_certificate_chain(tls_seq, conn_ctx, "filepath");
     //assert the crap out of it
     assert(y == 1);
     assert(conn_ctx.tls == "");
-    assert(|tls_opts_seq.opts_list| != 0);
-    assert(tls_opts_seq != null)
-    // assert(|tls_opts_seq.opts_list| >= old(|tls_opts_seq.opts_list|))
+    assert(|tls_seq.opts_list| != 0);
+    assert(tls_seq != null);
+    assert(|tls_seq.opts_list| >= old(|tls_seq.opts_list|));
+    sock.optsSeq := tls_seq;
 
     assert sock.Secure();
   }
